theories/LambdaBox_to_LambdaANF/anf_toplevel.v
@@ -1,0 +1,341 @@
+(* Top-level correctness theorems for ANF conversion from LambdaBox. *)
+
+From Stdlib Require Import ZArith.ZArith Lists.List micromega.Lia Arith
+     Ensembles Relations.Relation_Definitions.
+From MetaRocq.Erasure Require Import
+  EAst EAstUtils EGlobalEnv EWellformed EPrimitive.
+From MetaRocq.Common Require Import BasicAst Kernames.
+From compcert Require Import lib.Maps lib.Coqlib.
+From CertiRocq.Common Require Import AstCommon.
+From CertiRocq Require Import Pipeline_utils.
+From CertiRocq.LambdaANF Require Import
+  cps cps_show eval ctx logical_relations
+  List_util algebra alpha_conv functions Ensembles_util
+  tactics identifiers bounds cps_util rename set_util stemctx.
+From MetaRocq.Utils Require Import All_Forall.
+From CertiRocq.LambdaBox_to_LambdaANF Require Import
+  common ANF fuel_sem wf anf_corresp anf_util anf_correct anf_global.
+
+Import ListNotations.
+
+Section Refinement.
+
+  Context (func_tag kon_tag default_tag default_itag : positive)
+          (tgm : conId_map)
+          (cmap : const_map)
+          (cenv : ctor_env)
+          (Σ : EAst.global_context).
+
+  Context {efl : EEnvFlags}.
+  Context (HnoAxioms : has_axioms = false).
+
+  Context (dcon_to_tag_inj :
+    forall dc dc',
+      dcon_to_tag default_tag dc tgm = dcon_to_tag default_tag dc' tgm -> dc = dc').
+
+  Context (box_dc : dcon)
+          (box_tag : dcon_to_tag default_tag box_dc tgm = default_tag).
+
+  Context (cenv_case_consistent : forall P ctag, caseConsistent cenv P ctag).
+  Context (cmap_inj : forall k1 k2 v,
+    lookup_const cmap k1 = Some v ->
+    lookup_const cmap k2 = Some v -> k1 = k2).
+
+  Let Hf_src := LambdaBox_resource_fuel default_tag tgm box_dc box_tag.
+  Let Ht_src := LambdaBox_resource_trace default_tag tgm box_dc box_tag.
+
+  Let anf_val_rel' :=
+    @anf_val_rel func_tag default_tag tgm cmap nat Hf_src Ht_src Σ box_dc.
+  Let anf_env_rel0 :=
+    @anf_env_rel func_tag default_tag tgm cmap nat Hf_src Ht_src Σ box_dc.
+
+  Let global_env_rel' :=
+    @global_env_rel func_tag default_tag tgm cmap nat Hf_src Ht_src Σ box_dc.
+
+  Let src_eval := @eval_env_fuel nat Hf_src Ht_src Σ box_dc.
+  Let cmap_consistent' :=
+    @cmap_consistent cmap nat Hf_src Ht_src Σ box_dc.
+
+  Context (Hglob_term :
+    forall k decl body,
+      declared_constant Σ k decl ->
+      decl.(EAst.cst_body) = Some body ->
+      exists src_v f t, src_eval [] body (Val src_v) f t).
+
+  Context (Hglob_wf :
+    forall k decl body,
+      declared_constant Σ k decl ->
+      decl.(EAst.cst_body) = Some body ->
+      wellformed Σ 0 body = true).
+
+  Context (prim_map : M.t primitive)
+          (prims : list (primitive * positive)).
+  Context (Hwf_glob : wf_glob Σ).
+  Context (HnoVar : has_tVar = false)
+          (HnoEvar : has_tEvar = false)
+          (HnoCoFix : has_tCoFix = false)
+          (HnoLazy : has_tLazy_Force = false)
+          (Hblocks : cstr_as_blocks = true)
+          (HnoArray : has_primarray = false).
+  Context (no_prims : forall s, find_prim prims s = None).
+  Context (cmap_complete : forall s d,
+    lookup_constant Σ s = Some d -> lookup_const cmap s <> None).
+  Context (cmap_sound : forall k v,
+    lookup_const cmap k = Some v ->
+    exists decl body,
+      declared_constant Σ k decl /\ decl.(EAst.cst_body) = Some body).
+  Context (cmap_nodup_vals : NoDup (map snd cmap)).
+
+  Let val_rel_exists :=
+    @anf_val_rel_exists func_tag default_tag prim_map tgm prims cmap
+      _ Σ box_dc nat Hf_src Ht_src
+      Hglob_term Hwf_glob
+      HnoVar HnoEvar HnoCoFix HnoLazy Hblocks HnoArray
+      no_prims cmap_complete cmap_sound cmap_nodup_vals.
+
+  Fixpoint value_ref' (v1 : fuel_sem.value) (v2 : val) : Prop :=
+    let fix Forall2_aux vs1 vs2 :=
+        match vs1, vs2 with
+        | [], [] => True
+        | v1' :: vs1', v2' :: vs2' =>
+          value_ref' v1' v2' /\ Forall2_aux vs1' vs2'
+        | _, _ => False
+        end
+    in
+    match v1, v2 with
+    | fuel_sem.Con_v c1 vs1, Vconstr c2 vs2 =>
+      dcon_to_tag default_tag c1 tgm = c2 /\ Forall2_aux vs1 vs2
+    | fuel_sem.Clos_v _ _ _, Vfun _ _ _ => True
+    | fuel_sem.ClosFix_v _ _ _, Vfun _ _ _ => True
+    | _, _ => False
+    end.
+
+  Definition value_ref (v1 : fuel_sem.value) (v2 : val) : Prop :=
+    match v1, v2 with
+    | fuel_sem.Con_v c1 vs1, Vconstr c2 vs2 =>
+      dcon_to_tag default_tag c1 tgm = c2 /\ Forall2 value_ref' vs1 vs2
+    | fuel_sem.Clos_v _ _ _, Vfun _ _ _ => True
+    | fuel_sem.ClosFix_v _ _ _, Vfun _ _ _ => True
+    | _, _ => False
+    end.
+
+  Lemma value_ref_eq v1 v2 :
+    value_ref' v1 v2 <-> value_ref v1 v2.
+  Proof.
+    induction v1; try easy.
+
+    destruct v2; simpl; try easy.
+
+    revert l0. induction l; intros l'.
+    - split; intros [H1 H2]. split; eauto; destruct l'; eauto.
+      inv H2. split; eauto.
+    - split; intros [H1 H2].
+      + split; eauto. destruct l'; inv H2.
+        constructor; eauto. eapply IHl. split; eauto.
+      + split; eauto. destruct l'; inv H2.
+        constructor; eauto. eapply IHl. split; eauto.
+  Qed.
+
+  Definition refines (M : nat) (e_src : EAst.term) (e_tgt : exp) : Prop :=
+    forall (v_src : fuel_sem.value) (f_src t_src : nat),
+      src_eval [] e_src (Val v_src) f_src t_src ->
+      exists (v_tgt : val) (c_tgt : nat),
+        bstep_fuel cenv (M.empty val) e_tgt c_tgt (Res v_tgt) tt /\
+        (c_tgt <= t_src + M)%nat /\
+        value_ref v_src v_tgt.
+
+  Definition anf_rel_top (e : EAst.term) (Sg : Ensemble var) (e_tgt : exp) :=
+    exists Sg' S' C_env C r,
+      anf_cvt_rel_global func_tag default_tag tgm
+        Sg (List.rev Σ) [] cmap C_env Sg' /\
+      anf_cvt_rel func_tag default_tag tgm cmap
+        Sg' e [] S' C r /\
+      e_tgt = C_env |[ C |[ Ehalt r ]| ]|.
+
+  Lemma anf_val_comp k v1 v2 v3 :
+    anf_val_rel' v1 v2 ->
+    preord_val cenv eq_fuel k v2 v3 ->
+    value_ref v1 v3.
+  Proof.
+    revert v2 v3.
+    induction v1 using fuel_sem.value_ind'; intros v2 v3 Hval Hpre; inv Hval.
+    - rewrite preord_val_eq in Hpre.
+      destruct v3; try contradiction. inv Hpre.
+      simpl. split. reflexivity.
+
+      revert l vs' H2 H1.
+      induction H; intros.
+      + inv H2. inv H1. constructor.
+      + inv H2. inv H1. constructor; eauto.
+        eapply value_ref_eq. eauto.
+    - rewrite preord_val_eq in Hpre.
+      destruct v3; try contradiction.
+      simpl. exact I.
+    - rewrite preord_val_eq in Hpre.
+      destruct v3; try contradiction.
+      simpl. exact I.
+  Qed.
+
+  Theorem anf_correct_top_explicit e Sg Sg' S' C_env C r :
+    wellformed Σ 0 e = true ->
+    anf_cvt_rel_global func_tag default_tag tgm
+      Sg (List.rev Σ) [] cmap C_env Sg' ->
+    anf_cvt_rel func_tag default_tag tgm cmap
+      Sg' e [] S' C r ->
+    Disjoint _ (cmap_vars cmap) Sg ->
+    exists M, refines M e (C_env |[ C |[ Ehalt r ]| ]|).
+  Proof.
+    intros Hwf Hglob_cvt Hmain_cvt Hdis_glob.
+    destruct (@global_ctx_correct_top
+                func_tag kon_tag default_tag default_itag
+                tgm cmap cenv Σ efl
+                HnoAxioms
+                dcon_to_tag_inj
+                box_dc box_tag
+                cenv_case_consistent cmap_inj
+                Hglob_term Hglob_wf
+                prim_map prims Hwf_glob
+                HnoVar HnoEvar HnoCoFix HnoLazy Hblocks HnoArray
+                no_prims cmap_complete cmap_sound cmap_nodup_vals
+                C_env Sg Sg'
+                Hglob_cvt Hdis_glob (M.empty val))
+      as [rho_g [F_glob [T_glob [Hglob_rho Hpre_glob]]]].
+    exists (T_glob + 1).
+    intros src_v f t Heval.
+
+    pose proof (@anf_cvt_correct
+                  func_tag default_tag default_itag
+                  tgm cmap cenv Σ efl
+                  dcon_to_tag_inj
+                  box_dc box_tag
+                  cenv_case_consistent cmap_inj
+                  Hglob_term Hglob_wf
+                  prim_map prims Hwf_glob
+                  HnoVar HnoEvar HnoCoFix HnoLazy Hblocks HnoArray
+                  no_prims cmap_complete cmap_sound cmap_nodup_vals
+                  [] e (Val src_v) f t Heval)
+      as Hcorr.
+    unfold anf_cvt_correct_exp in Hcorr.
+
+    assert (Hwf_nil : well_formed_env Σ []) by constructor.
+    assert (Hcons_nil : env_consistent [] []).
+    { intros i j y Hi. destruct i; discriminate. }
+    assert (Hcmap_nil : cmap_consistent' [] []).
+    { intros i x k decl body Hi. destruct i; discriminate. }
+    assert (Hdis_nil : Disjoint _ (FromList []) Sg').
+    { rewrite FromList_nil. now apply Disjoint_Empty_set_l. }
+    assert (Hdis_main : Disjoint _ (cmap_vars cmap) Sg').
+    { eapply Disjoint_Included_r.
+      - eapply anf_cvt_global_subset. exact Hglob_cvt.
+      - exact Hdis_glob. }
+    assert (Henv_nil : anf_env_rel0 [] [] rho_g) by constructor.
+    assert (Hglob_main : global_env_rel' (kn_deps e) rho_g).
+    { intros k v Hdep Hlk.
+      eapply Hglob_rho.
+      - intro Hnone. rewrite Hlk in Hnone. discriminate.
+      - exact Hlk. }
+
+    specialize (Hcorr rho_g [] C r Sg' S' 1%nat
+                  Hwf_nil Hwf Hcons_nil Hcmap_nil
+                  Hdis_nil Hdis_main Henv_nil Hglob_main Hmain_cvt).
+
+    assert (Hdis_ehalt :
+      Disjoint _ (occurs_free (Ehalt r)) ((Sg' \\ S') \\ [set r])).
+    { rewrite occurs_free_Ehalt.
+      eapply Disjoint_Singleton_l.
+      intro Hin.
+      inv Hin.
+      match goal with
+      | [ Hnot : ~ _ \in [set _] |- _ ] => now apply Hnot; constructor
+      end. }
+
+    specialize (Hcorr (Ehalt r) Hdis_ehalt).
+    destruct Hcorr as [Hterm _].
+
+    assert (Hwf_src_v : well_formed_val Σ src_v).
+    { eapply eval_preserves_wf; [exact Hglob_wf | exact Hwf_nil | exact Hwf | exact Heval]. }
+    destruct (val_rel_exists src_v Hwf_src_v) as [v_anf Hrel_anf].
+    specialize (Hterm src_v v_anf eq_refl Hrel_anf).
+
+    assert (Hctx_main0 :
+      occurs_free_ctx C \subset FromList [] :|: (Sg' \\ S') :|: cmap_vars cmap).
+    { exact (@anf_cvt_occurs_free_ctx_exp
+               func_tag default_tag tgm cmap Σ box_dc box_tag
+               Sg' e [] S' C r Hmain_cvt Hdis_nil Hdis_main). }
+    assert (Hctx_main :
+      occurs_free_ctx C \subset (Sg' \\ S') :|: cmap_vars cmap).
+    { rewrite FromList_nil, Union_Empty_set_neut_l in Hctx_main0.
+      exact Hctx_main0. }
+
+    assert (Hr_not_old : ~ r \in (Sg \\ Sg')).
+    { intro Hin_old.
+      destruct (@anf_cvt_result_in_consumed
+                  func_tag default_tag tgm cmap
+                  Sg' e [] S' C r Hmain_cvt)
+        as [Hin_vn | [Hin_s | Hin_cm]].
+      - rewrite FromList_nil in Hin_vn. contradiction.
+      - exact ((proj2 Hin_old) Hin_s).
+      - eapply (Disjoint_In_l _ _ _ Hdis_glob Hin_cm). exact (proj1 Hin_old). }
+
+    assert (Hdis_cont :
+      Disjoint _ (occurs_free (C |[ Ehalt r ]|)) (Sg \\ Sg')).
+    { eapply Disjoint_Included_l.
+      - eapply occurs_free_ctx_app.
+      - eapply Union_Disjoint_l.
+        + eapply Disjoint_Included_l.
+	          * exact Hctx_main.
+	          * eapply Union_Disjoint_l.
+	            -- constructor. intros z Hz. inv Hz.
+	               match goal with
+	               | [ Hleft : z \in (Sg' \\ S'), Hright : z \in (Sg \\ Sg') |- _ ] =>
+	                 inv Hleft; inv Hright; contradiction
+	               end.
+	            -- eapply Disjoint_Included_r.
+	               ++ eapply Setminus_Included.
+	               ++ exact Hdis_glob.
+        + eapply Disjoint_Included_l.
+          * rewrite occurs_free_Ehalt. eapply Setminus_Included.
+          * eapply Disjoint_Singleton_l. exact Hr_not_old. }
+
+	    assert (Hpre_full :
+	      preord_exp cenv (comp (anf_bound f t) (anf_bound F_glob T_glob))
+	        eq_fuel 1
+	        (Ehalt r, M.set r v_anf rho_g)
+	        (C_env |[ C |[ Ehalt r ]| ]|, M.empty val)).
+	    { eapply preord_exp_trans; [tci | exact eq_fuel_idemp | | ].
+	      - exact Hterm.
+	      - intros m. exact (Hpre_glob (C |[ Ehalt r ]|) m Hdis_cont). }
+
+	    assert (Hehalt :
+	      bstep_fuel cenv (M.set r v_anf rho_g) (Ehalt r)
+	        (<0> <+> (<1> (Ehalt r))) (Res v_anf) (<0> <+> (<1> (Ehalt r)))).
+    { econstructor 2. econstructor. rewrite M.gss. reflexivity. }
+	    assert (Hle_halt : (to_nat (<0> <+> (<1> (Ehalt r))) <= 1)%nat).
+	    { simpl. unfold algebra.one, one_i. simpl. lia. }
+
+	    destruct (Hpre_full (Res v_anf) (<0> <+> (<1> (Ehalt r))) (<0> <+> (<1> (Ehalt r)))
+	               Hle_halt Hehalt)
+	      as [res_fin [c_fin [cout_fin [Hstep_fin [Hbound Hres_fin]]]]].
+	    destruct res_fin; try contradiction.
+	    destruct Hbound as [mid_cfg [Hbound_main Hbound_glob]].
+	    destruct mid_cfg as [[[e_mid rho_mid] c_mid] t_mid].
+	    unfold anf_bound in Hbound_main, Hbound_glob.
+	    simpl in Hbound_main, Hbound_glob.
+	    destruct cout_fin.
+
+	    exists v, c_fin. split; [exact Hstep_fin |]. split.
+	    - lia.
+	    - eapply anf_val_comp; eauto.
+  Qed.
+
+  Theorem anf_correct_top e Sg e_tgt :
+    wellformed Σ 0 e = true ->
+    Disjoint _ (cmap_vars cmap) Sg ->
+    anf_rel_top e Sg e_tgt ->
+    exists M, refines M e e_tgt.
+  Proof.
+    intros Hwf Hdis [Sg' [S' [C_env [C [r [Hglob [Hmain ->]]]]]]].
+    eapply anf_correct_top_explicit; eauto.
+  Qed.
+
+End Refinement.
